Examples/temp_cfi.v
@@ -1,0 +1,780 @@
+Require Import NArith ZArith Bool Coq.Lists.List.
+Require Import Lia ZifyBool ZifyN.
+Require Import -(notations) arm7_cfi2.
+Require Import Picinae_armv7.
+Require Import Lia ZifyN ZifyNat.
+Import ARM7Notations.
+Import ListNotations.
+Require Import Nat.
+
+Open Scope N.
+
+Definition to_a := Z.mul 4.
+Definition i2a' i2i' (i: Z) := to_a (i2i' i).
+Definition compute_table_size sr := Z.to_nat (2 ^ (32 - sr)).
+Definition compute_table_start_index tbi ti := Z.to_nat (ti - tbi).
+Definition SafeEntry i2i' (pol: Z -> list Z) ai si a :=
+  to_a ai = a \/ exists di (D: i2a' i2i' di = a), In di (pol si).
+Definition InBlock i ilen da' :=
+  (i * 4 <= Z.of_N da' < (i + Z.of_nat ilen) * 4 /\ N.divide 4 da')%Z.
+Definition SafeDest i2i' pol ai si ilen a :=
+  SafeEntry i2i' pol ai si (Z.of_N a) \/ InBlock (i2i' si) ilen a.
+Definition SafeTable i2i' pol ai si table :=
+  Forall (SafeEntry i2i' pol ai si) table.
+Definition extract_table sr tbi ti (flattened_tables: list Z) :=
+  let si := compute_table_start_index tbi ti in
+  let ts := compute_table_size sr in
+  let table := firstn ts (skipn si flattened_tables) in
+  if (si + ts <=? length flattened_tables)%nat && (tbi <=? ti)%Z then Some table else None.
+
+Definition ContainsBlock (p: program) b s i :=
+  forall i', InBlock i (length b) (i'*4) ->
+    match nth_error b (Z.to_nat (Z.of_N i' - i)) with
+    | Some z => p s (i'*4) = Some (4, arm2il (i'*4) (arm_decode z))
+    | None => False
+    end.
+Definition InBlockX i ilen (x: exit * store) :=
+  match fst x with
+  | Addr a => InBlock (Z.of_N i) ilen a
+  | _ => False
+  end.
+
+Lemma inblock_start {i ilen}: InBlock (Z.of_N i) (S ilen) (i*4).
+Proof.
+  split. lia. now exists i.
+Qed.
+Lemma inblockx_s:
+  forall i ilen x, InBlockX i ilen x /\ fst x <> Addr (i*4) -> InBlockX (i+1) (ilen-1) x.
+Proof.
+  unfold InBlockX. intros. destruct x, e. simpl in *.
+    destruct H as [[[? ?] [? ?]] ?]. repeat split; [destruct (N.eq_dec x i); [now subst | lia] | lia | now exists x].
+    easy.
+Qed.
+Lemma inblockx_cons:
+  forall i (b:Z) b' x,
+    InBlockX (i + 1) (length b') x -> InBlockX i (length (b :: b')) x.
+Proof.
+  intros. destruct x, e.
+    unfold InBlockX, InBlock in *. simpl in *. split. lia. easy.
+    easy.
+Qed.
+
+
+(* copied straight from the Z proof, since there is no N version for some reason *)
+Lemma Ndivdec a b : {(a | b)} + {~ (a | b)}.
+Proof.
+ destruct (N.eq_dec a 0) as [Ha|Ha].
+ - destruct (N.eq_dec b 0) as [Hb|Hb].
+   + left; subst; apply N.divide_0_r.
+   + right. subst. contradict Hb. now apply N.divide_0_l.
+ - destruct (N.eq_dec (b mod a) 0).
+   + left. now apply N.Lcm0.mod_divide.
+   + right. now rewrite <- N.Lcm0.mod_divide.
+Defined.
+Lemma inblockx_dec : forall i ilen a, {InBlockX i ilen a} + {~InBlockX i ilen a}.
+Proof.
+  intros. destruct a, e.
+  unfold InBlockX, InBlock. simpl.
+  destruct (Ndivdec 4 a), (Z_le_dec (Z.of_N i * 4) (Z.of_N a)), (Z_lt_dec (Z.of_N a) (((Z.of_N i) + Z.of_nat ilen) * 4)).
+  all: (now left) || (now right).
+Qed.
+
+(* for prog p that contains block b, after starting at entry index ei with store s,
+   prop P holds for all states constrained to the block as well as the first step outside the block *)
+Definition AfterBlock (P: exit * store -> Prop) b p s bi ei :=
+  forall t0 t1 a' s'
+    (XP: exec_prog p ((Addr a', s')::t1++t0))
+    (SO: ostartof t1 = Some (Addr (ei*4), s))
+    (CB: ContainsBlock p b s (Z.of_N bi))
+    (IB: Forall (InBlockX bi (length b)) t1),
+    P (Addr a', s').
+
+(* like AfterBlock, but ignores the first step outside the block *)
+Definition DuringBlock P b p s bi ei := AfterBlock (fun xs => P xs \/ ~InBlockX bi (length b) xs) b p s bi ei.
+(* an alternative definition that we prove is equivalent *)
+Definition DuringBlock' (P: _ -> Prop) b p s bi ei :=
+  forall t0 t1 a' s'
+    (XP: exec_prog p ((Addr a', s')::t1++t0))
+    (SO: ostartof t1 = Some (Addr (ei*4), s))
+    (CB: ContainsBlock p b s (Z.of_N bi))
+    (IB: Forall (InBlockX bi (length b)) ((Addr a', s')::t1)),
+    P (Addr a', s').
+Lemma db_db': forall P b p s bi ei, DuringBlock P b p s bi ei <-> DuringBlock' P b p s bi ei.
+Proof.
+  intros. unfold DuringBlock, DuringBlock', AfterBlock. split.
+    intros. apply H in XP. destruct XP. easy. now inversion IB. easy. easy. now inversion IB.
+    intros. destruct (inblockx_dec bi (length b) (Addr a', s')).
+      apply H in XP. now left. easy. easy. constructor. easy. easy.
+      now right.
+Qed.
+
+(* the given block does not change as long as we are still in the block
+
+   note that we use DuringBlock instead of AfterBlock,
+   since we need to assume this property to prove that blocks go to a safe destination,
+   but to prove that the block is maintained even after exiting the block,
+   we need to know that indirect jumps always load from the table *)
+Definition MaintainsBlock p b bi ei s :=
+  DuringBlock (fun xs => ContainsBlock p b (snd xs) (Z.of_N bi)) b p s bi ei.
+
+Lemma containsblock_cons:
+  forall p b b' s i, ContainsBlock p (b::b') s i -> ContainsBlock p b' s (i+1).
+Proof.
+  intros. unfold ContainsBlock, InBlock. intros. specialize (H i').
+  rewrite <-(Z.add_simpl_r i 1) in H at 2.
+  rewrite Z.sub_sub_distr, Z2Nat.inj_add, Nat.add_1_r, nth_error_S in H by lia. apply H.
+  simpl. split. lia. easy.
+Qed.
+
+Lemma ostartof_some_cons{A}:
+  forall a b (c:A), ostartof a = Some b -> ostartof (c::a) = Some b.
+Proof.
+  simpl. destruct a. easy. intros. now rewrite startof_cons.
+Qed.
+Lemma ostartof_last{A}:
+  forall a (b:A), ostartof a = Some b -> exists c, a = c ++ [b].
+Proof.
+  destruct a. easy. intros. destruct (@exists_last _ (a::a0)). easy. destruct s. exists x. rewrite e, ostartof_niltail in H. inversion H. now rewrite <-H1.
+Qed.
+Lemma single_element{A}:
+  forall (a: A) b c,
+    [a] = b ++ [c] ->
+    a = c.
+Proof.
+  intros. destruct b; simpl in H; inversion H; auto. now apply app_cons_not_nil in H2.
+Qed.
+Lemma forall_last{A}:
+  forall (P: A -> Prop) y x1 t1 t2 x2,
+    y::x1::t1 = t2 ++ [x2] ->
+    Forall P (x1::t1) ->
+    P x2.
+Proof.
+  intros. destruct (exists_last (ltac:(discriminate):x1::t1<>[])) as [? [? ?]].
+  rewrite e, app_comm_cons, app_inj_tail_iff in H. destruct H. subst.
+  rewrite e, Forall_app in H0. destruct H0. now inversion H0.
+Qed.
+
+
+(* if there is at least one element in l where P holds,
+   we can split l into two lists where the first does not have any such element,
+   and the second list starts with one *)
+Lemma exsplit{A}{P: A -> Prop}:
+  (forall a, {P a}+{~P a}) ->
+  forall l, Exists P l -> exists l1 x l2, l = l1 ++ x :: l2 /\ P x /\ ~(Exists P l1).
+Proof.
+  induction l. easy.
+  intros. destruct (X a).
+    exists nil, a, l. now subst.
+    rewrite Exists_cons in H. destruct H.
+      contradiction.
+      apply IHl in H as [? [? [? [? [? ?]]]]]. rewrite H. exists (a::x), x0, x1. repeat split; auto.
+      rewrite Exists_cons. unfold not. now rewrite Decidable.not_or_iff.
+Qed.
+Lemma cons_cons{A}: forall (a:A) b c, a::b::c = [a;b]++c. Proof. easy. Qed.
+Lemma app_cons{A}: forall (a:A) b c, c++a::b = (c++[a])++b.
+Proof.
+  intros. now rewrite <-app_assoc, <-app_comm_cons, app_nil_l.
+Qed.
+Lemma undofst{A}{B}:
+  forall (x: A * B) a,
+    fst x = a ->
+    exists b, x = (a,b).
+Proof.
+  intros. destruct x. exists b. now subst.
+Qed.
+
+(* if the initial store does not matter,
+   we only need to consider traces that do not contain the entry more than once to prove AfterBlock *)
+Lemma afterblock_noloop:
+  (forall P b p s bi ei,
+    (forall t0 t1 t2 t3 t4 a' s0 s'
+      (* the trace through the block does not loop back to the entry *)
+      (NL: ~ Exists (fun x => fst x = Addr (ei*4)) t1)
+      (* the store we start with is reachable by some trace through the block *)
+      (RA: s = s0 \/ (Forall (InBlockX bi (length b)) t3 /\ exec_prog p (t4++(Addr (ei*4), s0)::t3++(Addr (ei*4), s)::t2)))
+
+      (XP: exec_prog p ((Addr a', s')::t1++(Addr (ei*4), s0)::t0))
+      (CB: ContainsBlock p b s (Z.of_N bi))
+      (IB: Forall (InBlockX bi (length b)) t1),
+      P (Addr a', s')) ->
+    AfterBlock P b p s bi ei)%N.
+Proof.
+  intros. unfold AfterBlock. intros.
+  assert (forall x: exit * store, {fst x = Addr (ei*4)} + {fst x <> Addr (ei*4)}) by repeat decide equality.
+  destruct (Exists_dec _ t1 X).
+  - apply (exsplit X) in e as [? [? [? [? [? ?]]]]]. apply undofst in H1 as [? ?]. subst.
+      rewrite <-app_assoc in XP. apply Forall_app in IB as [? ?].
+      rewrite ostartof_app in SO. apply ostartof_last in SO as [? ?]. destruct x0.
+      + inversion H3. eapply (H t0 x nil nil nil). apply H2. now left. subst. apply XP. assumption. assumption.
+      + rewrite H3 in XP. eapply H. apply H2. right. inversion H3. subst.
+        rewrite <-app_assoc, app_comm_cons in XP. split. inversion H1. apply Forall_app in H7 as [? ?]. apply H7.
+        apply XP. inversion H3. subst. apply XP. assumption. assumption.
+  - apply ostartof_last in SO as [? ?]. subst. exfalso. apply n. apply Exists_app. right. now constructor.
+Qed.
+Lemma afterblock_impl:
+  forall P Q p b s bi ei
+    (I: forall x, P x -> Q x)
+    (AB: AfterBlock P p b s bi ei),
+    AfterBlock Q p b s bi ei.
+Proof.
+  unfold AfterBlock. intros. apply I. eapply AB. apply XP. all: easy.
+Qed.
+
+Lemma afterblock_suffix{P b p s bi ei ei' s' t0 t2}:
+  forall t1
+    (AB: AfterBlock P b p s bi ei)
+    (XP: exec_prog p (t2++(Addr (ei'*4), s')::t1++t0))
+    (SO: ostartof t1 = Some (Addr (ei * 4), s))
+    (CB: ContainsBlock p b s (Z.of_N bi))
+    (IB: Forall (InBlockX bi (length b)) t1),
+    AfterBlock P b p s' bi ei'.
+Proof.
+  intros; unfold AfterBlock; intros.
+  eapply (AB t0 (t4++t1)).
+  - rewrite <-app_assoc, app_comm_cons. rewrite app_cons in XP. apply exec_prog_split in XP as [? [? ?]]. apply exec_prog_app.
+      easy.
+      unfold can_step_between in *. destruct app eqn:e; auto. erewrite ostartof_some_cons. rewrite ostartof_niltail in H0. apply H0.
+      easy.
+      rewrite app_comm_cons in XP0. now apply exec_prog_split in XP0.
+  - apply ostartof_last in SO as [? ?]. now rewrite H, app_assoc, ostartof_niltail.
+  - now destruct t4.
+  - now rewrite Forall_app.
+Qed.
+Lemma xp_splice:
+  forall p t t' x, exec_prog p (x::t) -> exec_prog p t' -> ostartof t' = Some x -> exec_prog p (t'++t).
+Proof.
+  intros. apply exec_prog_app. now apply exec_prog_tail in H. unfold can_step_between. destruct t. easy. rewrite H1. now inversion H. easy.
+Qed.
+
+(* for a block b that is maintained through the entire execution through b, where the instruction at our entry index is z, if
+      1) z falls through to z' inside the block, P is true for this step, and P always holds after executing from z'
+      2) z goes to a state outside the block where P holds
+   or 3) z raises an exception
+   then P always holds after b if we start at z *)
+Lemma afterblock_step:
+  forall p b z s bi ei P
+    (MB: MaintainsBlock p b bi ei s)
+    (E: bi <= ei)
+    (Z: nth_error b (Z.to_nat (Z.of_N ei - Z.of_N bi)) = Some z),
+    (forall c' s s' x, exec_stmt armc s (arm2il (ei*4) (arm_decode z)) c' s' x ->
+      (* case 1 *)
+        (x = None /\
+        (MaintainsBlock p b bi (ei+1) (reset_temps s s') -> AfterBlock P b p (reset_temps s s') bi (ei+1)) /\
+        P (Addr ((ei+1)*4), (reset_temps s s'))) \/
+      (* case 2 (fallthru) *)
+        (x = None /\
+        length b = 1%nat /\
+        P (Addr ((ei+1)*4), (reset_temps s s'))) \/
+      (* case 2 (jump) *)
+        (exists a, x = Some (Addr a) /\
+        P (Addr a, (reset_temps s s')) /\
+        ~ (InBlock (Z.of_N bi) (length b) a)) \/
+      (* case 3 *)
+        (exists a, x = Some (Raise a))) ->
+    AfterBlock P b p s bi ei.
+Proof.
+  intros. unfold AfterBlock. intros.
+  specialize (CB ei) as CB'. rewrite Z in CB'.
+  remember (Z.to_nat _). pose proof (proj1 (nth_error_Some b n) ltac:(now rewrite Z)).
+  assert (InBlock (Z.of_N bi) (length b) (ei*4)) as IB' by (split; [lia|now exists ei]).
+  specialize (CB' IB').
+  apply ostartof_last in SO as [? ?]. rewrite H1, 2 app_comm_cons in XP.
+  destruct (@exists_last _ ((Addr a', s')::x) ltac:(discriminate)) as [? [? ?]]. rewrite e, <-2app_assoc in XP.
+  assert (XP':=XP). apply exec_prog_split in XP as [XP _]. simpl in XP.
+  inversion XP. inversion H4. rewrite CB' in LU. inversion LU. subst. apply H in XS.
+  clear H4 H5 LU H. destruct XS as [[? [? ?]]|[[? [? ?]]|[[? [? [? ?]]]|[? ?]]]]; subst;
+    (destruct x; [ apply single_element in e; inversion e; now try rewrite N.mul_add_distr_r in H2|]).
+  {
+    eapply H1.
+    eapply (afterblock_suffix [_] MB); [ rewrite N.mul_add_distr_r, app_nil_l; apply XP | now try constructor .. ].
+    rewrite app_assoc, <-e in XP'. simpl in XP'. rewrite app_comm_cons in XP'. apply XP'.
+    now erewrite <-ostartof_app, <-app_cons, app_nil_l, e, ostartof_app, N.mul_add_distr_r.
+    apply db_db' in MB. eapply MB; [rewrite <-app_cons, app_nil_l; apply XP| auto .. ];
+      apply (forall_last (InBlockX bi (length b))) in e;
+        [apply (Forall_cons _ e); constructor; now try apply IB'|].
+    all: now apply Forall_app in IB.
+  }
+  all: apply (forall_last (InBlockX bi (length b))) in e;
+    unfold InBlockX, InBlock in e; simpl in e; [now try lia|now apply Forall_app in IB].
+Qed.
+
+(* like afterblock_step, but we can forget about the first instruction of the block *)
+Lemma afterblock_cons:
+  forall p b b' s i P
+    (MB: MaintainsBlock p (b::b') i i s),
+    (forall c' s s' x, exec_stmt armc s (arm2il (i*4) (arm_decode b)) c' s' x ->
+      (* case 1 *)
+        (x = None /\
+        (MaintainsBlock p b' (i+1) (i+1) (reset_temps s s') -> AfterBlock P b' p (reset_temps s s') (i+1) (i+1)) /\
+        P (Addr ((i+1)*4), (reset_temps s s'))) \/
+      (* case 2 (fallthru) *)
+        (x = None /\
+        b' = nil /\
+        P (Addr ((i+1)*4), (reset_temps s s'))) \/
+      (* case 2 (jump) *)
+        (exists a, x = Some (Addr a) /\
+        P (Addr a, (reset_temps s s')) /\
+        ~ (InBlock (Z.of_N i) (length (b::b')) a)) \/
+      (* case 3 *)
+        (exists a, x = Some (Raise a))) ->
+    AfterBlock P (b::b') p s i i.
+Proof.
+  (* todo: clean this proof up *)
+  intros. apply afterblock_noloop.
+  intros. assert (XP':=XP). assert(CB':=CB). rewrite app_comm_cons in XP.
+  remember (_::t1). destruct (@exists_last _ l ltac:(now subst)) as [? [? ?]]. subst.
+  rewrite e, <-app_assoc in XP. simpl in XP. apply exec_prog_split in XP as [XP _]. inversion XP. clear x1 l H3 H0 H1. inversion H2. clear H2. subst.
+  assert (Some(sz, q) = p s (i*4)).
+  { destruct RA. now rewrite H0. destruct H0. unfold MaintainsBlock, DuringBlock in MB. specialize (MB t2 (t3++[(Addr (i*4), s)])).
+    simpl in MB. rewrite <-app_assoc in MB. simpl in MB. apply exec_prog_split in H1 as [? _]. eapply MB in H1. shelve. now rewrite ostartof_niltail. easy. apply Forall_app. split. easy. constructor. apply inblock_start. easy. Unshelve. destruct H1.
+    specialize (CB i (inblock_start)). specialize (H1 i (inblock_start)). rewrite Z.sub_diag, nth_error_O in CB, H1. simpl in CB, H1. now rewrite <-LU, H1, CB. exfalso.  apply H1. apply inblock_start.
+    }
+  specialize (CB i (inblock_start )). rewrite Z.sub_diag, nth_error_O in CB. simpl in CB. rewrite CB in H0. inversion H0.
+  subst. apply H in XS. destruct XS as [?|[?|[?|?]]].
+  shelve.
+  - destruct H1 as [? [? ?]]. destruct t1. apply single_element in e. inversion e. subst. rewrite H5. now rewrite N.mul_add_distr_r in H3.
+    apply forall_last with (P:=InBlockX i (length (b::b'))) in e.
+    subst. simpl in e. unfold InBlockX in e. simpl in e. unfold InBlock in e. lia. easy.
+  - destruct H1 as [? [? [? ?]]]. destruct t1. apply single_element in e. inversion e. subst. now rewrite H5.
+    apply forall_last with (P:=InBlockX i (length (b::b'))) in e.
+    subst. simpl in e. unfold InBlockX in e. simpl in e. contradiction. easy.
+  - destruct H1. subst. destruct t1. apply single_element in e. easy.
+    apply forall_last with (P:=InBlockX i (length (b::b'))) in e. easy. easy.
+    Unshelve.
+    destruct H1 as [? [? ?]].
+
+
+    destruct t1. apply single_element in e. inversion e. rewrite H5. subst. simpl.  rewrite N.mul_add_distr_r in H3. easy.
+    subst; simpl in *. eapply H2. shelve. rewrite 2 app_comm_cons in XP'. apply XP'. now erewrite <-ostartof_app, <-app_cons, app_nil_l, e, ostartof_app, N.mul_add_distr_r. rewrite N2Z.inj_add. eapply containsblock_cons. remember (_::_::_). replace l with
+      ([(Addr (i * 4 + 4), reset_temps s0 s'0) ; (Addr (i * 4), s0)] ++ t0)%N in XP. destruct RA. apply db_db' in MB. eapply MB. apply XP. now rewrite e0. easy. 
+      apply forall_last with (P:=InBlockX i (length (b::b'))) in e. constructor. assumption. constructor. apply inblock_start. easy. assumption. apply db_db' in MB. eapply MB.
+      destruct a. apply exec_prog_split in e0 as [? _]. apply exec_prog_split in XP as [_ [_ ?]]. 
+
+      enough (exec_prog p (([(Addr (i * 4 + 4), reset_temps s0 s'0);(Addr (i * 4), s0)]++t3++[(Addr (i*4), s)])++t2)). apply H5. rewrite <-app_assoc.
+      apply exec_prog_app. rewrite <-app_cons. now apply exec_prog_tail in H1. unfold can_step_between. simpl. rewrite <-app_assoc. destruct app; auto. now inversion H1. easy. simpl. now rewrite startof_niltail. assumption.
+    apply forall_last with (P:=InBlockX i (length (b::b'))) in e. constructor. easy. constructor. apply inblock_start. apply Forall_app. split. easy. constructor. apply inblock_start. easy. easy.
+      eapply Forall_impl. replace (length b') with ((length (b::b'))-1)%nat. apply inblockx_s. simpl. lia. apply Forall_Exists_neg in NL. now apply Forall_and.
+      Unshelve.
+      clear H NL CB H0 H2 H3 LU. apply db_db'. apply db_db' in MB. unfold DuringBlock', DuringBlock in *. intros. rewrite N2Z.inj_add. eapply containsblock_cons.
+      destruct RA; eapply MB; rewrite app_comm_cons in XP0; apply exec_prog_split in XP0 as [_ [_ ?]]; pose proof (xp_splice _ _ _ _ XP H); eapply ostartof_some_cons in SO; rewrite N.mul_add_distr_r in SO; apply H0 in SO. rewrite <-app_comm_cons, app_cons in SO. apply SO. now rewrite ostartof_niltail, e0. assumption.
+      rewrite app_comm_cons, Forall_app. split. eapply Forall_impl in IB0. apply IB0. apply inblockx_cons. constructor. apply inblock_start. easy.
+      destruct a. apply exec_prog_split in e0 as [? _]. rewrite <-app_comm_cons, app_cons , app_comm_cons in SO. apply exec_prog_split in SO as [_ [_ ?]].  pose proof (xp_splice _ _ _ _ H1 H2). rewrite app_comm_cons, ostartof_niltail, <-app_comm_cons, (app_cons (_, s)) in H3. 
+      rewrite <-app_comm_cons, (app_assoc (t6++_)) in H3. apply (H3 eq_refl). now rewrite app_assoc, ostartof_niltail. assumption. constructor.
+      apply inblockx_cons. now inversion IB0. repeat (rewrite Forall_app; split). eapply Forall_impl. apply inblockx_cons. now inversion IB0. constructor. apply inblock_start. easy. easy. constructor. apply inblock_start. easy.
+Qed.
+
+Definition SafeDestX i2i' pol ai si ilen (xs: exit * store) :=
+  match fst xs with
+  | Addr a => SafeDest i2i' pol ai si ilen a
+  | _ => False
+  end.
+
+
+Lemma forget_cond:
+  forall c s q1 e q2 q3 c' s' x,
+    exec_stmt c s (q1 $; If e q2 q3) c' s' x ->
+    exec_stmt c s (q1 $; If (Unknown 1) q2 q3) c' s' x.
+Proof.
+  intros. inversion H.
+    now constructor.
+    subst. eapply XSeq2.
+      apply XS1.
+      inversion XS0. destruct b; [apply XIf with (b:=0)|apply XIf with (b:=1)]; now try constructor.
+Qed.
+
+Ltac destruct_match_in H :=
+  repeat match type of H with context[match ?x with _ => _ end] =>
+    let e := fresh "e" in
+    destruct x eqn:e
+  end.
+Ltac destruct_match_eqn :=
+repeat match goal with |- context[match ?x with _ => _ end] =>
+    let e := fresh "e" in
+    destruct x eqn:e
+  end.
+Lemma arm_assemble_all_first:
+  forall a a' z,
+    arm_assemble_all (a::a') = Some z ->
+    exists h t, arm_assemble_all a' = Some t /\ z = h::t /\ arm_decode h = a.
+Proof.
+  induction z. intros. unfold arm_assemble_all in H. destruct_match_in H; discriminate. intros. exists a0, z. repeat split; unfold arm_assemble_all in H; destruct_match_in H; try discriminate. inversion H. now subst. apply arm_assemble_eq in e. inversion H. now subst.
+Qed.
+Lemma arm_assemble_all_len:
+  forall a b, arm_assemble_all a = Some b -> length a = length b.
+Proof.
+  intros. apply arm_assemble_all_eq in H. now rewrite <- H, length_map.
+Qed.
+Lemma arm_assemble_all_cond_len:
+  forall a cond b, arm_assemble_all_cond a cond = Some b -> (length a <= length b <= S (length a))%nat.
+Proof.
+  intros. unfold arm_assemble_all_cond in H. destruct Z.ltb. apply arm_assemble_all_len in H. rewrite <- H. simpl. lia. apply arm_assemble_all_eq in H. rewrite <- H, length_map. lia.
+Qed.
+Lemma afterblock_cond:
+  forall P b p s i l cond
+  (B: arm_assemble_all_cond l cond = Some b)
+  (I: i < 2^30 - 64)
+  (L: (1 <= length l < 64)%nat)
+  (MB: MaintainsBlock p b i i s)
+  (AB: match arm_assemble_all l with
+       | Some b' => forall s,
+           MaintainsBlock p b' (i + N.of_nat (length b - length b')) (i + N.of_nat (length b - length b')) s ->
+           AfterBlock P b' p s (i + N.of_nat (length b - length b')) (i + N.of_nat (length b - length b'))
+       | _ => True
+       end)
+  (PA: forall s, P (Addr ((i + N.of_nat (length b))*4), s))
+  (PS: forall s, P (Addr ((i + 1)*4), s)),
+    AfterBlock P b p s i i.
+Proof.
+  intros.
+
+  unfold arm_assemble_all_cond in B. destruct Z.ltb. 
+    apply arm_assemble_all_first in B as [? [? [? [? ?]]]]. subst.
+    apply afterblock_cons. assumption. intros.
+    rewrite H1 in H0.
+    cbv[arm2il arm_b_il BranchWritePC arm_R] in H0. apply forget_cond in H0. remember (i*4). remember (scast _ _ _). step_stmt H0.
+    destruct N.modulo; destruct H0 as [H0 _]; step_stmt H0; destruct H0 as [[_ ?] _].
+
+      left. repeat split. assumption. simpl length in AB. rewrite H, Nat.sub_succ_l, Nat.sub_diag in AB. intro. apply AB. assumption. lia. easy.
+
+      assert (n ⊕ 8 ⊕ n0 .& 4294967292 = (i + N.of_nat (S(length l)))*4) as E.
+      {
+        subst.
+        rewrite N.mul_add_distr_r, N.shiftl_mul_pow2. rewrite <-Z_nat_N, Z2Nat.inj_sub, Nat2Z.id, Nat2N.inj_sub, Z_nat_N by easy.
+        cbn. rewrite N.mul_sub_distr_r. unfold scast. epose proof (proj1 (toZ_nonneg _ _)). rewrite H0.
+        rewrite (N.mod_small _ (2^26)), N2Z.inj_sub, N2Z.inj_mul, nat_N_Z by lia. cbn. unfold ofZ. rewrite Z2N.inj_mod by lia. replace (Z.to_N (_ - _)) with (N.of_nat (length l) * 4 - 4) by lia. rewrite <-N.Div0.add_mod.
+        change 4294967296 with (2^32). rewrite N_land_mod_pow2_move by lia.
+        change (4294967292 mod 2 ^ 32) with (N.lnot (2 * (2 * 0 + 1) + 1) 32).
+        rewrite <- N.ldiff_land_low, 2 N.ldiff_odd_r, N.ldiff_0_r. lia. apply N.log2_lt_pow2. lia. lia. enough (N.of_nat (length l) * 4 - 4 < 2^ 25). rewrite N.mod_small by lia. apply H2. lia.
+      }
+      simpl length in PA. apply arm_assemble_all_len in H.
+      right. right. left. repeat esplit. apply H0. rewrite E, H. apply PA.
+      unfold InBlock. rewrite E. simpl length. lia.
+
+   rewrite B, Nat.sub_diag, N.add_0_r in AB. apply AB, MB.
+Qed.
+
+
+Lemma afterblock_fallthru:
+  forall P b b' p s bi, Forall (fun z => forall s c' s' x i a, exec_stmt armc s (arm2il i (arm_decode z)) c' s' x -> x <> Some (Addr a)) (b++[b']) ->
+  (forall a s, InBlock (Z.of_N bi) (length (b++[b'])) a -> P (Addr a, s)) ->
+  (MaintainsBlock p (b++[b']) bi bi s) ->
+  (forall s, P (Addr ((bi + N.of_nat (length (b++[b'])))*4), s)) -> AfterBlock P (b++[b']) p s bi bi.
+Proof.
+  induction b. - intros. simpl. apply afterblock_cons. simpl in H0. assumption. intros. destruct x. destruct e. inversion H. apply (H6 _ _ _ _ _ a) in H3. contradiction.
+  right. right. right. now exists i. right. left. repeat split. apply H2.
+  - simpl. intros. apply afterblock_cons. assumption. intros. destruct x. destruct e. inversion H. apply (H6 _ _ _ _ _ a0) in H3. contradiction.
+  right. right. right. now exists i. left. repeat split. intro. apply IHb. inversion H. assumption. intros. apply H0. unfold InBlock in *. split. lia. easy. assumption.
+  remember (length _). 
+  Search (_ + N.of_nat _). intros. 
+  rewrite <-(N2Nat.id 1), <-N.add_assoc, <- Nat2N.inj_add. apply H2. apply H0. split. rewrite length_app. simpl. lia. apply N.divide_factor_r.
+Qed.
+Lemma afterblock_fallthru':
+  forall P b p s bi, Forall (fun z => forall s c' s' x i a, exec_stmt armc s (arm2il i (arm_decode z)) c' s' x -> x <> Some (Addr a)) b -> 
+  (forall a s, InBlock (Z.of_N bi) (length b) a -> P (Addr a, s)) ->
+  (1 <= length b)%nat ->
+  (MaintainsBlock p b bi bi s) ->
+  (forall s, P (Addr ((bi + N.of_nat (length b))*4), s)) -> AfterBlock P b p s bi bi.
+Proof.
+  intros. destruct b. now simpl in H1. destruct (exists_last (ltac:(discriminate):z::b<>[])) as [? [? ?]]. rewrite e in *. now apply afterblock_fallthru.
+Qed.
+
+
+Lemma GOTO_correct:
+  forall s l src dest c' s' x i,
+    src < 2^30 ->
+    dest < 2^30 ->
+    GOTO l 14 (Z.of_N src) (Z.of_N dest) = Some i ->
+    exec_stmt armc s (arm2il (src * 4) i) c' s' x ->
+    x = Some (Addr (dest * 4)).
+Proof.
+  intros s l src dest c' s' x i S D G. intros.
+  cbv [GOTO] in G. destruct orb eqn:e in G; try discriminate.
+  remember (_ - _ - _)%Z as offset. unfold Z2 in *.
+  assert (src * 4 ⊕ 8 ⊕ scast 26 32 (Z.to_N (offset mod 16777216) << 2) .& 4294967292 = dest * 4).
+  {
+    change 2 with (Z.to_N 2) at 2. rewrite <- Z2N_inj_shiftl, Z.shiftl_mul_pow2, <- Zmult_mod_distr_r by lia.
+    change (Z.to_N _) with (ofZ 26 (offset * 4)).
+    unfold scast. rewrite toZ_ofZ by (unfold signed_range; cbn; lia). unfold ofZ.
+    rewrite <- (N2Z.id ((_ + 8) mod _)), <- Z2N.inj_add, N2Z.inj_mod, <- (N2Z.id (_ ^ _)), <- Z2N.inj_mod, <- Zplus_mod by lia.
+    replace (_ + _ * 4)%Z with (Z.of_N (dest * 4)) by lia.
+    rewrite Z2N.inj_mod, 2 N2Z.id, N_land_mod_pow2_move by lia.
+    change (_ mod _) with (N.lnot (2 * (2 * 0 + 1) + 1) 32).
+    rewrite <- N.ldiff_land_low, 2 N.ldiff_odd_r, N.ldiff_0_r. lia.
+    destruct (dest * 4) eqn:E; now try solve [apply N.log2_lt_pow2; lia].
+  }
+  destruct l; inversion G; subst; cbv [arm2il arm_bl_il arm_b_il] in H;
+    remember (scast _ _ _) as dsta; remember (src * 4) as srca;
+    step_stmt H; destruct H as [H _];
+    step_stmt H; destruct H as [[_ ?] _]; now rewrite H, H0.
+Qed.
+
+Lemma GOTOz_correct:
+  forall s l src dest c' s' x z,
+    src < 2^30 ->
+    dest < 2^30 ->
+    GOTOz l 14 (Z.of_N src) (Z.of_N dest) = Some z ->
+    exec_stmt armc s (arm2il (src * 4) (arm_decode z)) c' s' x ->
+    x = Some (Addr (dest * 4)).
+Proof.
+  intros. unfold GOTOz in H1. destruct GOTO eqn:e in H1; try discriminate. apply arm_assemble_eq in H1. rewrite H1 in H2.
+  now apply (GOTO_correct s l src dest c' s' x a).
+Qed.
+
+Definition NoJ q := forall_stmts_in_stmt (fun q' : stmt => forall e : exp, q' <> Jmp e) q.
+Definition NoE q := forall_stmts_in_stmt (fun q' : stmt => forall i : N, q' <> Exn i) q.
+Definition NoJE q := NoJ q /\ NoE q.
+Lemma noj_cond: forall cond il, NoJ il -> NoJ (arm_cond_il cond il).
+Proof. easy. Qed.
+Lemma noj_seq: forall a b, NoJ a -> NoJ b -> NoJ (a $; b).
+Proof. easy. Qed.
+Lemma noje_cond: forall cond il, NoJE il -> NoJE (arm_cond_il cond il).
+Proof. intros. destruct H. easy. Qed.
+Lemma noje_seq: forall a b, NoJE a -> NoJE b -> NoJE (a $; b).
+Proof. intros. now destruct H, H0. Qed.
+Lemma noj_ite: forall a b c, NoJ a -> NoJ b -> NoJ (If c b a).
+Proof. easy. Qed.
+
+Lemma arm_cond_fallthru:
+  forall cond il c s c' s' x
+    (XS: exec_stmt c s (arm_cond_il cond il) c' s' x),
+    (forall x', exec_stmt c s il c' s' x' -> x' = None) ->
+    x = None.
+Proof.
+  intros. cbv [arm_cond_il] in XS. destruct_match_in XS; first
+    [ now apply H in XS
+    | inversion XS; destruct b; first [now apply H in XS0 | now inversion XS0]].
+Qed.
+Local Ltac noje H :=
+  match type of H with
+  | exec_stmt _ _ (arm2il ?a ?i) _ _ ?x =>
+      let A := fresh "A" in
+      let B := fresh "B" in
+      assert (NoJE (arm2il a i)) as [A B]; [cbv [arm2il]; apply noje_seq; [split;discriminate|try apply noje_cond] | now apply stmt_xnone in H]
+  end.
+Local Ltac noj H :=
+  match type of H with
+  | exec_stmt _ _ (arm2il ?a ?i) _ _ ?x =>
+      let A := fresh "A" in
+      assert (NoJ (arm2il a i)) as A; [cbv [arm2il]; apply noj_seq; [discriminate|try apply noj_cond] | eapply stmt_xnotaddr; now try apply H]
+  end.
+Local Ltac nje :=
+  repeat match goal with
+  | |- NoJE (arm_cond_il _ _) => apply noje_cond
+  | |- NoJE (Seq _ _) => apply noje_seq
+  | |- NoJE ?a => unfold_rec a
+  end; try (split;discriminate).
+Ltac nj :=
+  repeat match goal with
+  | |- NoJ (arm_cond_il _ _) => apply noj_cond
+  | |- NoJ (Seq _ _) => apply noj_seq
+  | |- NoJ ?a => unfold_rec a
+  end.
+Lemma for_0_14_noj:
+  forall reg_list start f,
+    NoJ start -> (forall n, NoJ (f n)) -> NoJ (for_0_14 reg_list start f).
+Proof.
+  intros. repeat apply noj_seq; destruct_match_eqn; apply H0 || discriminate || assumption.
+Qed.
+Lemma arm_lsm_noj:
+  forall op cond W Rn register_list a c s c' s' x A
+    (XS: exec_stmt c s (arm2il a (ARM_lsm op cond W Rn register_list)) c' s' x),
+    (Z.to_N register_list < 2 ^ 15 -> x <> Some (Addr A))%N.
+Proof.
+  (* intros. noj XS; cbv[arm_lsm_il arm_lsm_op_il arm_lsm_op_type arm_stm_il arm_ldm_il arm_lsm_il_]. easy. time (destruct_match_eqn; *)
+  (* nj; try solve [eapply xbits_above in H; rewrite H in e0; lia]; apply noj_ite; now try apply for_0_14_noj). *)
+Admitted. (*speed this up*)
+Lemma arm_data_r_fallthru:
+  forall op cond S Rn Rd imm5 type Rm a c s c' s' x
+    (XS: exec_stmt c s (arm2il a (ARM_data_r op cond S Rn Rd imm5 type Rm)) c' s' x),
+    Rd <> 15%Z -> x = None.
+Proof.
+  intros. noje XS.
+  cbv[arm_data_r_il arm_data_op_il arm_data_r_shiftc arm_data_r_addwcarry arm_data_il].
+  destruct DecodeImmShift, Shift_C. destruct_match_eqn; try lia; nje.
+Qed.
+Lemma arm_data_i_fallthru:
+  forall op cond S Rn Rd imm12 a c s c' s' x
+    (XS: exec_stmt c s (arm2il a (ARM_data_i op cond S Rn Rd imm12)) c' s' x),
+    Rd <> 15%Z -> x = None.
+Proof.
+  intros. noje XS.
+  cbv[arm_data_i_il arm_data_op_il arm_data_i_shiftc arm_data_i_addwcarry arm_data_il].
+  destruct ARMExpandImm_C. destruct_match_eqn; try lia; nje.
+Qed.
+Lemma arm_ls_i_fallthru:
+  forall op cond P U W Rn Rt imm12 a c s c' s' x
+    (XS: exec_stmt c s (arm2il a (ARM_ls_i op cond P U W Rn Rt imm12)) c' s' x),
+    Rt <> 15%Z \/ op <> ARM_LDR -> x = None.
+Proof.
+  intros. noje XS.
+  cbv [arm_ls_i_il arm_ls_op_il arm_ls_il]. destruct H; destruct_match_eqn; try lia; nje; contradiction || (repeat split; try discriminate).
+Qed.
+Lemma arm_ls_r_fallthru:
+  forall op cond P U W Rn Rt imm5 type Rm a c s c' s' x
+    (XS: exec_stmt c s (arm2il a (ARM_ls_r op cond P U W Rn Rt imm5 type Rm)) c' s' x),
+    Rt <> 15%Z \/ op <> ARM_LDR -> x = None.
+Proof.
+  intros. noje XS.
+  cbv [arm_ls_r_il arm_ls_op_il arm_ls_il]. destruct H; destruct_match_eqn; try lia; nje; contradiction || (repeat split; try discriminate).
+Qed.
+Lemma arm_movwt_fallthru:
+  forall is_w cond imm4 Rd imm12 a c s c' s' x
+    (XS: exec_stmt c s (arm2il a (ARM_MOV_WT is_w cond imm4 Rd imm12)) c' s' x),
+    x = None.
+Proof.
+  intros; noje XS; destruct is_w; split; discriminate.
+Qed.
+
+Lemma In_contains:
+  forall z l, contains z l = true -> In z l.
+Proof.
+  intros. unfold contains in H. destruct_match_in H; try discriminate. apply find_some in e. destruct e. apply Z.eqb_eq in H1. now subst.
+Qed.
+Lemma arm_lsm_reglist_bound:
+  forall reg reg2,
+    (0 <= reg < 15)%Z ->
+    (0 <= reg2 < 15)%Z ->
+  Z.to_N (Z.lor (Z.shiftl 1 reg) (Z.shiftl 1 reg2)) < 2 ^ 15.
+Proof.
+  intros. rewrite Z2N_inj_lor by now apply Z.shiftl_nonneg.
+  apply lor_bound; (rewrite Z2N_inj_shiftl, N.shiftl_mul_pow2, N.mul_1_l; [apply N.pow_lt_mono_r| |] ; lia).
+Qed.
+Lemma unused_reg_not_pc:
+  forall base r0 r1 r2, (base < 12 -> _unused_reg base r0 r1 r2 <> 15)%Z.
+Proof.
+  intros. unfold _unused_reg, Z1, Z2, Z3. destruct_match_eqn; lia.
+Qed.
+Lemma unused_reg_bound:
+  forall base r0 r1 r2, (0 <= base < 12 -> 0 <= _unused_reg base r0 r1 r2 < 15)%Z.
+Proof.
+  intros. unfold _unused_reg, Z1, Z2, Z3. destruct_match_eqn; lia.
+Qed.
+
+Local Ltac ft XS :=
+  unfold LDR, STR, MOV, MOVW, MOVT in XS; match type of XS with
+  | context[ARM_data_i] => eapply arm_data_i_fallthru in XS; [subst;discriminate | try apply unused_reg_not_pc;unfold Z4;lia]
+  | context[ARM_data_r] => eapply arm_data_r_fallthru in XS; [subst;discriminate | try apply unused_reg_not_pc;unfold Z4;lia]
+  | context[ARM_ls_i] => eapply arm_ls_i_fallthru in XS; [subst;discriminate | (left;apply unused_reg_not_pc;unfold Z4;lia) || lia || now right]
+  | context[ARM_ls_r] => eapply arm_ls_r_fallthru in XS; [subst;discriminate | (left;apply unused_reg_not_pc;unfold Z4;lia) || lia || now right]
+  | context[ARM_lsm] => eapply arm_lsm_noj in XS; [apply XS|simpl Z.shiftl in *;lia]
+  | context[STMDB2] => eapply arm_lsm_noj in XS; [apply XS|apply arm_lsm_reglist_bound; try apply unused_reg_bound;unfold Z4;lia]
+  | context[LDMDB2] => eapply arm_lsm_noj in XS; [apply XS|apply arm_lsm_reglist_bound; try apply unused_reg_bound;unfold Z4;lia]
+  | _ => noj XS; unfold arm_assign_MemU, arm_R; destruct_match_eqn; repeat split; try discriminate; easy
+  end.
+Local Ltac faft :=
+  repeat constructor; solve [intros ?????? XS; ft XS] || assumption || idtac.
+
+Definition SafeAfterBlock i2i' pol ai i irm p s := AfterBlock (SafeDestX i2i' pol ai i (length irm)) irm p s (Z.to_N (i2i' i)) (Z.to_N (i2i' i)).
+Lemma SafeDest_rewrite_inst:
+  forall tc i2i' z pol i ti ai bi txt irm' table tc' p s1
+    (TC: True) (* table cache is consistent with memory *)
+    (AI: (0 <= ai < 2^30)%Z)
+    (TI: (0 <= ti < 2^30)%Z)
+    (I:  (0 <=  i < 2^30)%Z)
+    (BI: (0 <= bi < 2^30)%Z)
+    (AIB: ~ InBlock (i2i' i) (length irm') (Z.to_N ai * 4))
+    (I2I': (0 <= i2i' i < 2^30)%Z)
+    (I2I'': (i2i' (i + 1) = i2i' i + Z.of_nat (length irm'))%Z)
+    (RI: rewrite_inst tc i2i' z (pol i) i ti ai bi txt = Some (irm', table, tc'))
+    (MB: MaintainsBlock p irm' (Z.to_N (i2i' i)) (Z.to_N (i2i' i)) s1),
+
+    SafeAfterBlock i2i' pol ai i irm' p s1.
+Proof.
+  intros.
+
+  assert (
+    forall l cond, arm_assemble_all_cond l cond = Some irm' ->
+      (1 <= length l < 64)%nat ->
+      In (Z.add i 1) (pol i) ->
+      match arm_assemble_all l with
+      | Some b' => forall s,
+        MaintainsBlock p b'
+          (Z.to_N (i2i' i) + N.of_nat (length irm' - length b'))
+          (Z.to_N (i2i' i) + N.of_nat (length irm' - length b')) s ->
+        AfterBlock (SafeDestX i2i' pol ai i (length irm')) b' p s
+          (Z.to_N (i2i' i) + N.of_nat (length irm' - length b'))
+          (Z.to_N (i2i' i) + N.of_nat (length irm' - length b'))
+      | None => True
+      end ->
+    SafeAfterBlock i2i' pol ai i irm' p s1
+  ) as C. {
+    intros. eapply afterblock_cond. apply H. admit. assumption. assumption. assumption. 
+      intros. unfold SafeDestX, SafeDest. simpl. left. right. exists (i+1)%Z. split. unfold i2a', to_a. lia. assumption.
+      intros. unfold SafeDestX, SafeDest. simpl. 
+      destruct (Nat.eq_dec (length irm') 1). left. right. exists(i+1)%Z. split. unfold i2a', to_a. lia. assumption.
+      right. unfold InBlock. split. split. lia.
+      apply arm_assemble_all_cond_len in H.
+      lia. apply N.divide_factor_r.
+  }
+  assert (
+    forall l cond, arm_assemble_all_cond l cond = Some irm' ->
+      (Forall (fun q => forall s c' s' x i a, exec_stmt armc s (arm2il i q) c' s' x  -> x <> Some (Addr a)) l) ->
+      (1 <= length l < 64)%nat ->
+      In (Z.add i 1) (pol i) ->
+    SafeAfterBlock i2i' pol ai i irm' p s1
+  ) as FT. {
+    intros. eapply C. apply H. assumption. assumption.
+    destruct arm_assemble_all eqn:e; auto.
+    intros. apply afterblock_fallthru'.
+      apply arm_assemble_all_eq in e. rewrite <-e, Forall_map in H0. assumption.
+      intros. cbv[SafeDestX fst]. right.
+        rewrite N2Z.inj_add, Z2N.id, nat_N_Z in H4 by lia. apply arm_assemble_all_cond_len in H.  apply arm_assemble_all_len in e.
+        remember (_ - _)%nat. assert (n = 0 \/ n = 1)%nat. destruct n. now left. right.  lia. destruct H5. replace (length irm') with (length l0) by lia. now rewrite H5, Z.add_0_r in H4. unfold InBlock in *. split. lia. easy. apply arm_assemble_all_len in e. lia.
+        assumption.
+        intros. cbv[SafeDestX fst SafeDest]. left. right. exists (i+1)%Z. split. unfold i2a', to_a. rewrite <- N.add_assoc, <- Nat2N.inj_add, <-Nat.sub_sub_distr, Nat.sub_diag, Nat.sub_0_r, I2I''. lia. lia. apply arm_assemble_all_cond_len in H. apply arm_assemble_all_len in e. lia. assumption.
+  }
+
+  assert (
+    forall sanitized_inst cond reg tc,
+      rewrite_pc_no_jump sanitized_inst cond i reg tc = Some (irm', table, tc') ->
+      (forall s c' s' x i a, exec_stmt armc s (arm2il i sanitized_inst) c' s' x  -> x <> Some (Addr a)) ->
+      reg <> 15%Z ->
+      In (Z.add i 1) (pol i) ->
+    SafeAfterBlock i2i' pol ai i irm' p s1
+  ) as RPNJ. {
+    intros. eapply FT. unfold rewrite_pc_no_jump, wo_table in H. destruct_match_in H; try discriminate.
+    inversion H. subst. apply e. faft. simpl. lia. assumption.
+  }
+  assert (
+    forall sanitized_inst cond reg reg2 tc,
+      rewrite_pc_sp_no_jump sanitized_inst cond i reg reg2 tc = Some (irm', table, tc') ->
+      (forall s c' s' x i a, exec_stmt armc s (arm2il i sanitized_inst) c' s' x  -> x <> Some (Addr a)) ->
+      (0 <= reg < 15)%Z ->
+      (0 <= reg2 < 15)%Z ->
+      In (Z.add i 1) (pol i) ->
+    SafeAfterBlock i2i' pol ai i irm' p s1
+  ) as RPSNJ. {
+    intros. eapply FT. unfold rewrite_pc_sp_no_jump, wo_table in H. destruct_match_in H; try discriminate.
+    inversion H. subst. apply e. faft. simpl. lia. assumption.
+  }
+  assert (goto_abort (i2i' i) ai tc = Some (irm', table, tc') -> SafeAfterBlock i2i' pol ai i irm' p s1) as GA.
+  {
+    intros. unfold goto_abort in H; destruct_match_in H; try discriminate. inversion H; subst.
+    apply afterblock_cons. assumption. intros. right. right. left. rewrite <-(Z2N.id (i2i' i)), <-(Z2N.id ai) in e by (apply I2I' || lia).
+    eapply GOTOz_correct in e. exists (Z.to_N ai * 4). repeat split. apply e. unfold SafeDestX. simpl. left. left. unfold to_a. lia. now rewrite Z2N.id by apply I2I'. lia. lia. apply H0.
+  }
+  assert (
+    irm' = [z] ->
+    In (Z.add i 1) (pol i) ->
+    (forall c s c' s' x a, exec_stmt c s (arm2il (Z.to_N (i2i' i) * 4) (arm_decode z)) c' s' x -> x <> Some (Addr a)) ->
+    SafeAfterBlock i2i' pol ai i irm' p s1
+  ) as FTS. {
+    intros. subst.
+    apply afterblock_cons. assumption. intros.
+    destruct x eqn:e. destruct e0. now eapply H1 in H. right. right. right. now exists i0. right. left. split. easy. split. easy.
+    unfold SafeDestX, SafeDest. simpl. left. right. exists (Z.add i 1). split. unfold i2a', to_a. rewrite N2Z.inj_mul, N2Z.inj_add, Z2N.id, I2I'', Z.mul_comm. easy.
+    apply I2I'. assumption.
+  }
+
+  unfold rewrite_inst, PC, Z1, Z15 in RI. destruct_match_in RI; try discriminate;
+  match type of RI with
+  | context[goto_abort] => now apply GA
+  | context[Some ([z], _, _)] => apply FTS; [now inversion RI| rewrite negb_false_iff in e; now apply In_contains in e|faft]
+  | context[rewrite_mov_lr_pc]=>
+    unfold rewrite_mov_lr_pc, wo_table in RI; destruct_match_in RI; try discriminate; inversion RI; subst; eapply FT; [apply e4|faft| simpl; lia|rewrite negb_false_iff in e; now apply In_contains in e]
+  | context[wo_table]=>
+    unfold wo_table in RI; destruct_match_in RI; try discriminate; inversion RI; subst; eapply FT; [apply e6|faft| simpl; lia|rewrite negb_false_iff in e; now apply In_contains in e]
+  | context[rewrite_pc_no_jump] => eapply RPNJ; [apply RI|faft|try apply unused_reg_not_pc;easy ..|rewrite negb_false_iff in e;now apply In_contains in e]
+  | context[rewrite_pc_sp_no_jump]=> eapply RPSNJ; [apply RI|faft|try apply unused_reg_bound;easy ..|rewrite negb_false_iff in e;now apply In_contains in e]
+  | _ => clear C GA FT FTS RPNJ RPSNJ
+  end.
